fixtures/TypeChecker.mli
@@ -1519,6 +1519,12 @@ val check_fn_root_shadow_no_capture_direct_call_component_store_safe_summary_wit
 val check_env_root_shadow_no_capture_direct_call_component_store_safe_summary_with_local_bounds_narrow_summary :
   global_env -> bool
 
+val check_fn_root_shadow_no_capture_direct_call_component_store_safe_summary_with_ready_body_or_local_narrow_summary :
+  global_env -> fn_def -> bool
+
+val check_env_root_shadow_no_capture_direct_call_component_store_safe_summary_with_ready_body_or_local_narrow_summary :
+  global_env -> bool
+
 val check_fn_root_shadow_direct_receiver_method_or_no_capture_direct_component_store_safe_summary :
   global_env -> fn_def -> bool
 
@@ -1663,6 +1669,9 @@ val check_env_root_shadow_no_receiver_component_narrow_summary_provider_check :
   global_env -> bool
 
 val check_env_root_shadow_no_receiver_component_local_bounds_narrow_summary_provider_check :
+  global_env -> bool
+
+val check_env_root_shadow_no_receiver_component_ready_body_or_local_narrow_summary_provider_check :
   global_env -> bool
 
 val check_env_root_shadow_no_receiver_component_ready_body_summary_provider_check_with_shadow_checks :
